cfrontend/Cshmgenproof.v
@@ -1420,23 +1420,23 @@ Inductive match_cont: composite_env -> type -> nat -> nat -> Clight.cont -> Csha
       match_cont ce tyret 0%nat (S ncnt)
                  (Clight.Kswitch k)
                  (Kblock tk)
-  | match_Kcall: forall ce tyret nbrk ncnt nbrk' ncnt' f e k id tf te le cp tk cu,
+  | match_Kcall: forall ce tyret nbrk ncnt nbrk' ncnt' f e k id tf te le tk cu,
       linkorder cu prog ->
       transl_function cu.(prog_comp_env) f = OK tf ->
       match_env e te ->
       match_cont cu.(prog_comp_env) (Clight.fn_return f) nbrk' ncnt' k tk ->
       match_cont ce tyret nbrk ncnt
-                 (Clight.Kcall id f e le cp k)
-                 (Kcall id tf te le cp tk)
-  | match_Kcall_normalize: forall ce tyret nbrk ncnt nbrk' ncnt' f e k id a tf te le vf tk cu,
+                 (Clight.Kcall id f e le k)
+                 (Kcall id tf te le tk)
+  | match_Kcall_normalize: forall ce tyret nbrk ncnt nbrk' ncnt' f e k id a tf te le tk cu,
       linkorder cu prog ->
       transl_function cu.(prog_comp_env) f = OK tf ->
       match_env e te ->
       match_cont cu.(prog_comp_env) (Clight.fn_return f) nbrk' ncnt' k tk ->
       (forall v e le m, wt_val v tyret -> le!id = Some v -> eval_expr tge e (comp_of f) le m a v) ->
       match_cont ce tyret nbrk ncnt
-                 (Clight.Kcall (Some id) f e le vf k)
-                 (Kcall (Some id) tf te le vf (Kseq (Sset id a) tk)).
+                 (Clight.Kcall (Some id) f e le k)
+                 (Kcall (Some id) tf te le (Kseq (Sset id a) tk)).
 
 Inductive match_states: Clight.state -> Csharpminor.state -> Prop :=
   | match_state:
@@ -1459,11 +1459,11 @@ Inductive match_states: Clight.state -> Csharpminor.state -> Prop :=
       match_states (Clight.Callstate fd args k m)
                    (Callstate tfd args tk m)
   | match_returnstate:
-      forall res tres k m tk ce
+      forall res tres k m tk ce cp
           (MK: match_cont ce tres 0%nat 0%nat k tk)
           (WT: wt_val res tres),
-      match_states (Clight.Returnstate res k m)
-                   (Returnstate res tk m).
+      match_states (Clight.Returnstate res k m cp)
+                   (Returnstate res tk m cp).
 
 Remark match_states_skip:
   forall f e le te nbrk ncnt k tf tk m cu,
@@ -1680,7 +1680,6 @@ Proof.
     eapply allowed_call_translated; eauto.
     erewrite <- find_comp_translated, <- type_of_call_translated; eauto.
     econstructor; eauto.
-    rewrite (Genv.match_genvs_find_comp TRANSL).
     eapply match_Kcall with (ce := prog_comp_env cu') (cu := cu); eauto.
     exact I.
   + (* with normalization of return value *)
@@ -1696,7 +1695,6 @@ Proof.
     erewrite <- find_comp_translated, <- type_of_call_translated; eauto.
     traceEq.
     econstructor; eauto.
-    rewrite (Genv.match_genvs_find_comp TRANSL).
     eapply match_Kcall_normalize  with (ce := prog_comp_env cu') (cu := cu); eauto.
     intros. eapply make_normalization_correct; eauto. constructor; eauto.
     exact I.
@@ -1798,6 +1796,7 @@ Proof.
   apply plus_one. constructor.
   eapply match_env_free_blocks; eauto.
   rewrite <- (comp_transl_function _ _ _ TRF). eauto.
+  rewrite <- (comp_transl_function _ _ _ TRF).
   eapply match_returnstate with (ce := prog_comp_env cu); eauto.
   eapply match_cont_call_cont. eauto.
   constructor.
@@ -1810,6 +1809,7 @@ Proof.
   rewrite <- (comp_transl_function _ _ _ TRF). eauto.
   eapply match_env_free_blocks; eauto.
   rewrite <- (comp_transl_function _ _ _ TRF). eauto.
+  rewrite <- (comp_transl_function _ _ _ TRF).
   eapply match_returnstate with (ce := prog_comp_env cu); eauto.
   eapply match_cont_call_cont. eauto.
   apply wt_val_casted. eapply cast_val_is_casted; eauto.
@@ -1821,6 +1821,7 @@ Proof.
   apply plus_one. apply step_skip_call. auto.
   eapply match_env_free_blocks; eauto.
   rewrite <- (comp_transl_function _ _ _ TRF). eauto.
+  rewrite <- (comp_transl_function _ _ _ TRF).
   eapply match_returnstate with (ce := prog_comp_env cu); eauto.
   constructor.
 
@@ -1916,7 +1917,7 @@ Proof.
     rewrite <- type_of_call_translated with (f := f) (cu := cu); auto.
     econstructor. constructor.
     simpl.
-    rewrite <- (comp_transl_function _ _ _ H11). apply H14. eauto. apply PTree.gss.
+    rewrite <- (comp_transl_function _ _ _ H10). apply H13. eauto. apply PTree.gss.
     traceEq.
     simpl. rewrite PTree.set2. econstructor; eauto. simpl; reflexivity. constructor.
 Qed.
